## Definition
We define
$$
\begin{align}
\cosh (z) &= \frac{e^z - e^{-z}}{2} = \sum_{n\in \mathbb N} \frac{z^{2n}}{(2n)!}\\
\sinh (z) &= \frac{e^z - e^{-z}}{2i} = \sum_{n\in \mathbb N} \frac{z^{2n+1}}{(2n+1)!} \\
\end{align}
$$
## Properties
We get that:
$$
\begin{align}
\cosh(-z) &= \cosh(z) \tag{1} \\
\sinh(-z) &= -\sinh(z) \tag{2} \\
\cosh(z + 2\pi ik) &= \cosh(z) \tag{3} \\
\sinh(z + 2\pi ik) &= \sinh(z) \tag{4} \\
\cosh(x + y) &= \cosh(x)\cosh(y) + \sinh(x)\sinh(y) \tag {5} \\
\sinh(x + y) &= \cosh(x)\sinh(y) + \sinh(x)\cosh(y) \tag {6} \\
\cosh^2(z) - \sinh^2(z) &= 1 \tag {7} \\
\cosh(x + iy) &= \cosh(x)\cos(y) + i\sinh(x)\sin(y) \tag {8}\\
\sinh(x + iy) &= \sinh(x)\cos(y) + i\cosh(x)\sin(y) \tag {9}\\
\end{align}
$$
and that:
$$
\begin{align}
\cosh(ix) &= \cos(x) \\
\sinh(ix) &= i\sin(x)
\end{align}
$$
## Derivatives
We get the identities:
$$
\begin{align}
\frac{d}{dx}\cosh(x) &= \sinh(x) \tag{1} \\
\frac{d}{dx}\sinh(x) &= \cosh(x) \tag{2}
\end{align}
$$
