## Definition
We define
$$
\begin{align}
\cos (z) &= \frac{e^{iz} - e^{-iz}}{2} = \sum_{n\in \mathbb N} \frac{(-1)^nz^{2n}}{(2n)!}\\
\sin (z) &= \frac{e^{iz} - e^{-iz}}{2i} = \sum_{n\in \mathbb N} \frac{(-1)^nz^{2n+1}}{(2n+1)!} \\
\end{align}
$$
## Properties
We get that:
$$
\begin{align}
\cos(-z) &= \cos(z) \tag{1} \\
\sin(-z) &= -\sin(z) \tag{2} \\
\cos(z + 2\pi k) &= \cos(z) \tag{3} \\
\sin(z + 2\pi k) &= \sin(z) \tag{4} \\
\cos(z+w) &= \cos(z)\cos(w) - \sin(z)\sin(w) \tag {5} \\
\sin(z + w) &= \cos(z)\sin(w) + \sin(z)\cos(w) \tag {6} \\
\cos^2(z) + \sin^2(z) &= 1 \tag {7} \\
\end{align}
$$
Further we get the relationsips that:
$$
\begin{align}
\sin(iy) &= i\sinh(y) \\
\cos(ix) &= \cosh(y)
\end{align}
$$
## Derivatives
We get the identities:
$$
\begin{align}
\frac{d}{dx}\cos(x) &= -\sin(x) \tag{1} \\
\frac{d}{dx}\sin(x) &= \cos(x) \tag{2}
\end{align}
$$